<?xml version="1.0"?>
<!--
CRMinf v0.7a harmonised with CIDOC CRM v6.2.1 and CRMinf 1.2.3 encoded in RDFS

Created by ICS-FORTH (CCI-ISL-ICS) Wednesday 27 July 2016

Encoding Rules:
1. The RDF spelling rules do not allow blanks. Hence we have replaced them by underscores.
   The blank between the concept identifier and concept name is replaced by underscore too.
   For instance "I1_Argumentation" or "J2_concluded_that".

2. RDF does not allow to instantiate properties beginning from a range value.
   Therefore, each CRMinf property is represented as two RDFS properties.
   For instance "J2_concluded_that (was_concluded_by)" is represented as:
   "J2_concluded_that" for the domain to range direction and "J2i_was_concluded_by" for the range to domain direction.
   
3. The primitive value "I6 Belief Value"  referred in
   the Model for formal completeness is interpreted as rdf: literal.

4. RDF does not provide a way to declare equivalence between two classes. So the information that I5 Inference Making is
   equivalent to S5 Inference Making is lost.

5. Scope notes are represented as <rdf:comment> elements.

6. Any other differences in labels, scope notes  and semantic relationships of this encoding 
to the authoritative definition of the CRMinf v0.7a (February  2015) are not intended transfer errors. 
FORTH appreciates your feed-back on such errors.

-->
<rdf:RDF xml:lang="en" xmlns:rdf="http://www.w3.org/1999/02/22-rdf-syntax-ns#" xmlns:rdfs="http://www.w3.org/2000/01/rdf-schema#"
        xml:base="http://www.cidoc-crm.org/cidoc-crm/CRMinf/">
		
<rdfs:Class rdf:about="I1_Argumentation">
	<rdfs:label xml:lang="en">Argumentation</rdfs:label>
	<rdfs:comment>This class comprises the activity of making honest inferences or observations. An honest inference or observation is one in which the E39 Actor carrying out the I1 Argumentation justifies and believes that the I6 Belief Value associated with resulting I2 Belief about the I4 Proposition Set is the correct value at the time that the activity was undertaken and that any I3 Inference Logic  or methodology was correctly applied.
	Only one instance of E39 Actor may carry out an instance of I1 Argumentation, though the E39 Actor may, of course, be an instance of E74 Group.
</rdfs:comment>
	<rdfs:subClassOf rdf:resource="http://www.cidoc-crm.org/cidoc-crm/E13_Attribute_Assignment"/>
</rdfs:Class>

<rdfs:Class rdf:about="http://www.cidoc-crm.org/cidoc-crm/CRMsci/S4_Observation">
	<rdfs:subClassOf rdf:resource="I1_Argumentation"/>
</rdfs:Class>

<rdfs:Class rdf:about="http://www.cidoc-crm.org/cidoc-crm/CRMsci/S5_Inference_Making">
	<rdfs:subClassOf rdf:resource="I1_Argumentation"/>
</rdfs:Class>

<rdfs:Class rdf:about="I2_Belief">
	<rdfs:label xml:lang="en">Belief</rdfs:label>
	<rdfs:comment>This class comprises the notion that the associated I4 Proposition Set is held to have a particular I6 Belief Value by a particular E39 Actor. This can be understood as the period of time that an individual or group holds a particular set of propositions to be true, false or somewhere in between.</rdfs:comment>
	<rdfs:subClassOf rdf:resource="http://www.cidoc-crm.org/cidoc-crm/E2_Temporal_Entity"/>
</rdfs:Class>

<rdfs:Class rdf:about="I3_Inference_Logic">
	<rdfs:label xml:lang="en">Inference Logic</rdfs:label>
	<rdfs:comment>This class comprises the rules used as inputs to I5 Inference Making.
	In this context the term “logic” is used in the most general sense of the Greek term, and not in the mathematical sense only. Examples are the direct application of formal logic, mathematical theories and calculus, formal or informal default reasoning based on default values associated with categories, probabilistic reasoning based mathematical models and assumed or observed frequencies for certain categories, application of theoretical social models and comparisons with “cultural parallels”, etc. An instance of Inference Logic could also be a reference to the exact software release of a Bayesian reasoner, a rule such as “later layers are on top of earlier layers”, or even a term like “social intuition”, if this is scholarly acceptable. (after Doerr, Kritsotaki and Boutsika 2011). Indeed anything that is scientifically or academically acceptable as a method for drawing conclusions may be included for instance human pattern recognition.
	A particular instance of I3 Inference Logic would be the algorithm implemented in a particular revision of a software package.
	Instances of I3 Inference Logic not only comprise the method of reasoning, but also the set of categorical laws or axioms used in the argumentation. Often both are inextricably interwoven, for instance in a software implementation.
</rdfs:comment>
	<rdfs:subClassOf rdf:resource="http://www.cidoc-crm.org/cidoc-crm/E89_Propositional_Object"/>
</rdfs:Class>

<rdfs:Class rdf:about="I4_Proposition_Set">
	<rdfs:label xml:lang="en">Proposition Set</rdfs:label>
	<rdfs:comment>This class comprises the sets of formal, binary propositions that an I2 Belief is held about. It could be implemented as a named graph, a spreadsheet or any other structured data-set. Regardless of the specific syntax employed, the effective propositions it contains should be made up of unambiguous identifiers, concepts of a formal ontology and constructs of logic.</rdfs:comment>
	<rdfs:subClassOf rdf:resource="http://www.cidoc-crm.org/cidoc-crm/E73_Information_Object"/>
</rdfs:Class>

<rdfs:Class rdf:about="I5_Inference_Making">
	<rdfs:label xml:lang="en">Inference Making</rdfs:label>
	<rdfs:comment>This class comprises the action of making honest propositions and statements about particular states of affairs in reality or in possible realities or categorical descriptions of reality by using inferences from other statements based on hypotheses and any form of formal or informal logic. It includes evaluations, calculations, and interpretations based on mathematical formulations and propositions. 
	It is characterized by the use of an existing I2 Belief as the premise that together with a set of I3 Inference Logic draws a further I2 Belief as a conclusion.
	Documenting instances of I5 Inference Making primarily enables tracing the dependency of knowledge from conclusion to premise through subsequent inferences, possibly back to primary evidence, so that the range of influence of knowledge revision at any intermediate stage of complex inference chains on current convictions can be narrowed down by query. The explicit reference to the applied inference logic further allows scholars or scientists to assess if they can or would follow the documented argument. The class is not intended to promote the use of computationally decidable systems of logic as replacements of scholarly justifications of arguments, even though it allows for documenting the use of decidable logic, if that was deemed adequate for the problem at hand.  Principles of scholarly justifications of arguments are also regarded as kinds of inference logic.</rdfs:comment>
	<rdfs:subClassOf rdf:resource="I1_Argumentation"/>
</rdfs:Class>

<rdfs:Class  rdf:about="http://www.ics.forth.gr/isl/CRMsci/S6_Data_Evaluation">
	<rdfs:subClassOf rdf:resource="I5_Inference_Making"/>
</rdfs:Class>

<rdfs:Class  rdf:about="http://www.ics.forth.gr/isl/CRMsci/S7_Simulation_or_Prediction">
	<rdfs:subClassOf rdf:resource="I5_Inference_Making"/>
</rdfs:Class>

<rdfs:Class  rdf:about="http://www.ics.forth.gr/isl/CRMsci/S8_Categorical_Hypothesis_Building">
	<rdfs:subClassOf rdf:resource="I5_Inference_Making"/>
</rdfs:Class>

<rdfs:Class rdf:about="I7_Belief_Adoption">
	<rdfs:label xml:lang="en">Belief Adoption</rdfs:label>
	<rdfs:comment>This class comprises the action of an E39 Actor adopting a particular instance of I2 Belief to create a new instance of I2 Belief that shares some of the same propositions in the original I4 Proposition Set and the associated I6 Belief Value.
	The basis of I7 Belief Adoption is trust in the source of the instance of I2 Belief rather than the application of the rules in instances of I3 Inference Logic.
		Typical examples are the citation of academic papers or the reuse of data sets.
	Where an instance of I7 Belief Adoption is based on personal communication (pers.comm.) this should be represented by using P2 has type: “Pers.Comm.” directly from the instance of I7 Belief Adoption.</rdfs:comment>
	<rdfs:subClassOf rdf:resource="I1_Argumentation"/>
</rdfs:Class>

<rdf:Property rdf:about="J1_used_as_premise">
	<rdfs:label xml:lang="en">used as premise</rdfs:label>
	<rdfs:comment>This property associates an instance of I2 Belief with the instance of I5 Inference Making that used it as a premise.</rdfs:comment>
	<rdfs:domain rdf:resource="I5_Inference_Making"/>
	<rdfs:range rdf:resource="I2_Belief"/>
	<rdfs:subPropertyOf rdf:resource="http://www.cidoc-crm.org/cidoc-crm/P17_was_motivated_by"/>
</rdf:Property>

<rdf:Property rdf:about="J1i_was_premise_for">
	<rdfs:label xml:lang="en">was premise for</rdfs:label>
	<rdfs:domain rdf:resource="I2_Belief"/>
	<rdfs:range rdf:resource="I5_Inference_Making"/>
	<rdfs:subPropertyOf rdf:resource="http://www.cidoc-crm.org/cidoc-crm/P17i_motivated"/>
</rdf:Property>

<rdf:Property rdf:about="J2_concluded_that">
	<rdfs:label xml:lang="en">concluded that</rdfs:label>
	<rdfs:comment>This property associates an instance of I2 Belief with the instance of I1 Argumentation that concluded it.</rdfs:comment>
	<rdfs:domain rdf:resource="I1_Argumentation"/>
	<rdfs:range rdf:resource="I2_Belief"/>
	<rdfs:subPropertyOf rdf:resource="http://www.cidoc-crm.org/cidoc-crm/P116_starts"/>
</rdf:Property>

<rdf:Property rdf:about="J2i_was_concluded_by">
	<rdfs:label xml:lang="en">was concluded by</rdfs:label>
	<rdfs:domain rdf:resource="I2_Belief"/>
	<rdfs:range rdf:resource="I1_Argumentation"/>
	<rdfs:subPropertyOf rdf:resource="http://www.cidoc-crm.org/cidoc-crm/P116i_is_started_by"/>
</rdf:Property>

<rdf:Property rdf:about="J3_applies">
	<rdfs:label xml:lang="en">applies</rdfs:label>
	<rdfs:comment>This property associates an instance of I3 Inference Logic with the instance of I5 Inference Making that used it to draw its conclusion.</rdfs:comment>
	<rdfs:domain rdf:resource="I5_Inference_Making"/>
	<rdfs:range rdf:resource="I3_Inference_Logic"/>
	<rdfs:subPropertyOf rdf:resource="http://www.cidoc-crm.org/cidoc-crm/P16_used_specific_object"/>
</rdf:Property>

<rdf:Property rdf:about="J3i_was_applied_by">
	<rdfs:label xml:lang="en">was applied by</rdfs:label>
	<rdfs:domain rdf:resource="I3_Inference_Logic"/>
	<rdfs:range rdf:resource="I5_Inference_Making"/>
	<rdfs:subPropertyOf rdf:resource="http://www.cidoc-crm.org/cidoc-crm/P16i_was_used_for"/>
</rdf:Property>

<rdf:Property rdf:about="J4_that">
	<rdfs:label xml:lang="en">that</rdfs:label>
	<rdfs:comment>This property associates an instance of I4 Proposition Set with the instance of I2 Belief that holds an opinion about it.</rdfs:comment>
	<rdfs:domain rdf:resource="I2_Belief"/>
	<rdfs:range rdf:resource="I4_Proposition_Set"/>
</rdf:Property>

<rdf:Property rdf:about="J4i_is_subject_of">
	<rdfs:label xml:lang="en">is subject of</rdfs:label>
	<rdfs:domain rdf:resource="I4_Proposition_Set"/>
	<rdfs:range rdf:resource="I2_Belief"/>
</rdf:Property>

<rdf:Property rdf:about="J5_holds_to_be">
	<rdfs:label xml:lang="en">holds to be</rdfs:label>
	<rdfs:comment>This property associates an instance of I2 Belief with the I6 Belief Value that reflects the opinion of the instance of I2 Belief about the I4 Proposition Set associated with it.</rdfs:comment>
	<rdfs:domain rdf:resource="I2_Belief"/>
	<rdfs:range rdf:resource="http://www.w3.org/2000/01/rdf-schema#Literal"/>
</rdf:Property>

<rdf:Property rdf:about="J6_adopted">
	<rdfs:label xml:lang="en">adopted</rdfs:label>
	<rdfs:comment>This property associates an instance of I2 Belief with the instance of I7 Belief Adoption that used it as the source of the I6 Belief Value and propositions used in the resulting new I2 Belief.</rdfs:comment>
	<rdfs:domain rdf:resource="I7_Belief_Adoption"/>
	<rdfs:range rdf:resource="I2_Belief"/>
	<rdfs:subPropertyOf rdf:resource="http://www.cidoc-crm.org/cidoc-crm/P17_was_motivated_by"/>
</rdf:Property>

<rdf:Property rdf:about="J6i_adopted_by">
	<rdfs:label xml:lang="en">adopted by</rdfs:label>
	<rdfs:domain rdf:resource="I2_Belief"/>
	<rdfs:range rdf:resource="I7_Belief_Adoption"/>
	<rdfs:subPropertyOf rdf:resource="http://www.cidoc-crm.org/cidoc-crm/P17i_motivated"/>
</rdf:Property>

<rdf:Property rdf:about="J7_is_based_on_evidence_from">
	<rdfs:label xml:lang="en">is based on evidence from</rdfs:label>
	<rdfs:comment>This property associates an instance of I7 Belief Adoption with the instance of E73 Information Object that was the source of or evidence for the I4 Proposition Set that was adopted.</rdfs:comment>
	<rdfs:domain rdf:resource="I7_Belief_Adoption"/>
	<rdfs:range rdf:resource="http://www.cidoc-crm.org/cidoc-crm/E73_Information_Object"/>
	<rdfs:subPropertyOf rdf:resource="http://www.cidoc-crm.org/cidoc-crm/P16_used_specific_object"/>
</rdf:Property>

<rdf:Property rdf:about="J7i_is_evidence_for">
	<rdfs:label xml:lang="en">is evidence for</rdfs:label>
	<rdfs:domain rdf:resource="http://www.cidoc-crm.org/cidoc-crm/E73_Information_Object"/>
	<rdfs:range rdf:resource="I7_Belief_Adoption"/>
	<rdfs:subPropertyOf rdf:resource="http://www.cidoc-crm.org/cidoc-crm/P16i_was_used_for"/>
</rdf:Property>

</rdf:RDF>